General rope based on binary tree

rope.dfy
@@ -1,344 +1,58 @@
-module Rope {
-  const max: int
-  const min: int
-
-  datatype Node<T> = Leaf(value: T) | InternalNode(children: seq<Rope<T>>)
-
-  class Rope<T> {
-    var val: Node<T>
-    var len: int
-
-    constructor Init(v: T)
-    ensures pathHasLeaf()
-    {
-      val := Leaf(v);
-      len := 0;
-    }
-
-    predicate validNumbers()
-      reads this, match this.val case InternalNode(children) => validChildrenNumber.reads(children) case Leaf(v) => validChildrenNumber.reads([])
-    {
-      // valid root
-      match this.val
-      case Leaf(v) => true
-      case InternalNode(children) =>
-        |children| <= max && this.validChildrenNumber(children)
-    }
-
-    predicate validChildrenNumber(children: seq<Rope<T>>)
-      reads this, children
-      decreases |children|
-    {
-      if |children| == 0 then true
-      else
-        match children[0].val
-          case Leaf(v) => true
-          case InternalNode(c) => this.validChildrenNumber(children[1..])
-    }
-
-    predicate pathsHaveLeaves(c: seq<Rope<T>>)
-      reads c
-    {
-      if |c| == 0 then false
-      else
-        match c[0].val
-        case Leaf(v) => true
-        case InternalNode(children) => pathsHaveLeaves(c[1..])
-    }
-
-    predicate pathHasLeaf()
-      reads this, match this.val case InternalNode(children) => pathsHaveLeaves.reads(children) case Leaf(v) => pathsHaveLeaves.reads([])
-      decreases this.val
-    {
-      match this.val
-      case Leaf(v) => true
-      case InternalNode(children) => this.pathsHaveLeaves(children)
-    }
-  }
-}
+// Basically a binary tree with Strings as leaves and len
+// Based on https://github.com/Microsoft/dafny/blob/master/Test/dafny1/BinaryTree.dfy
 
 
-----
+datatype Node = Leaf(value: string) | InternalNode(left: Rope, right: Rope)
 
-
-
-module Rope {
-  datatype Node<T> = Leaf(value: T) | InternalNode(children: seq<Rope<T>>)
-
-  class Rope<T> {
-    var val: Node<T>
-    var len: int
-    var max: int
-    var min: int
-
-
-    function sum<T>(c: seq<Rope<T>>): int
-      requires |c| > 0
-    {
-      if |c| == 1 then countLeaves(c[0])
-      else countLeaves(c[0]) + sum(c[1..])
-    }
-
-
-    function countLeaves(r: Rope): int
-      decreases r
-    {
-      match r
-      case Leaf(v) => 1
-      case Node(children) =>
-        if |children| <= 0 then 0
-        else sum(children)
-    }
-  }
-}
-
-
-class Node {
-  ghost var Contents: set<int>
+class Rope {
   ghost var Repr: set<object>
+  ghost var Content: set<string>
 
-  var data: int
-  var nodes: set<Node>
+  var len: int
+  var val: Node
+
+  constructor Init(v: string)
+  ensures Valid()
+  ensures ValidLen()
+  {
+    val := Leaf(v);
+    len := |v|;
+    Repr := {this};
+    Content := {v};
+  }
+
+  function Len(): int
+    requires Valid()
+    reads Repr
+    decreases Repr
+  {
+    match this.val
+    case Leaf(v) => |v|
+    case InternalNode(left, right) => left.Len() + right.Len()
+  }
+
+  predicate ValidLen()
+    requires Valid()
+    reads this, Repr
+  {
+    match this.val
+    case Leaf(v) => this.len == |v|
+    case InternalNode(left, right) => this.len == left.Len()
+  }
 
   predicate Valid()
     reads this, Repr
   {
     this in Repr &&
-    (|nodes| > 0 ==>
-      forall n :: n in nodes ==> n in Repr && n.Repr <= Repr && this !in n.Repr && n.Valid()
-    ) &&
-    (|nodes| == 0 ==>
-      Contents == {data})
-  }
-}
-
-
-module Rope {
-  datatype Node<T> = Leaf(value: T) | InternalNode(children: seq<Rope<T>>)
-
-  class Rope<T> {
-    var val: Node<T>
-    var len: int
-    var max: int
-    var min: int
-
-
-    function sum<T>(c: seq<Rope<T>>): int
-      reads c
-      requires |c| > 0
-      decreases c
-    {
-      if |c| == 1 then c[0].countLeaves()
-      else c[0].countLeaves() + sum(c[1..])
-    }
-
-
-    function countLeaves(): int
-      reads this
-      decreases this.val
-    {
+    (
       match this.val
-      case Leaf(v) => 1
-      case InternalNode(children) =>
-        if |children| <= 0 then 0
-        else this.sum(children)
-    }
+      case Leaf(v) => true
+      case InternalNode(left, right) =>
+        left != null && right != null &&
+        left in this.Repr && right in this.Repr &&
+        this !in left.Repr && this !in right.Repr &&
+        this.Repr >= left.Repr && this.Repr >= right.Repr &&
+        left.Valid() && right.Valid()
+    )
   }
-}
-
-
-
-
-
-predicate validChildren(rope: Rope<T>)
-  reads rope
-{
-  match rope.val
-  case Leaf(t) => true    // todo: all children must be either leaves or internal nodes? not mixed?
-  case InternalNode(children) => |children| >= min && |children| <= max && forall k: int :: 0 <= k < |children| ==> validChildren(children[k])
-}
-
-
-
-
-predicate childCount(rope: Rope<T>)
-  reads rope
-{
-  match rope.val
-  case Leaf(t) => true
-  case InternalNode(children) => forall k: int :: 0 <= k < children.Length ==> minChildren(a[k])
-}
-
-
-
-
-datatype Rope<T> = Leaf(value: T) | Node(children: seq<Rope<T>>)
-
-function sum<T>(c: seq<Rope<T>>): int
-  requires |c| > 0
-{
-  if |c| == 1 then countLeaves(c[0])
-  else countLeaves(c[0]) + sum(c[1..])
-}
-
-
-function countLeaves(r: Rope): int
-  decreases r
-{
-  match r
-  case Leaf(v) => 1
-  case Node(children) =>
-    if |children| <= 0 then 0
-    else sum(children)
-}
-
-
-
-module Rope {
-  datatype Node<T> = Leaf(value: T) | InternalNode(children: seq<Rope<T>>)
-
-  class Rope<T> {
-    var val: Node<T>
-    var len: int
-    var max: int
-    var min: int
-
-    function sum<T>(c: seq<Rope<T>>): int
-      reads c
-      decreases |c|
-    {
-      if |c| == 0 then 0
-      else if |c| == 1 then c[0].countLeaves()
-      else c[0].countLeaves() + sum(c[1..])
-    }
-
-
-    function countLeaves(): int
-      reads this
-      decreases this
-    {
-      match this.val
-      case Leaf(v) => 1
-      case InternalNode(children) => sum(children)
-    }
-  }
-}
-
-
-module Rope {
-  datatype Node<T> = Leaf(value: T) | InternalNode(children: seq<Rope<T>>)
-
-  class Rope<T> {
-    var val: Node<T>
-    var len: int
-    var max: int
-    var min: int
-
-    predicate childCount(rope: Rope<T>)
-      reads rope
-    {
-      match rope.val
-      case Leaf(t) => true
-      case InternalNode(children) => forall k: int :: 0 <= k < |rope.val.children| ==> minChildren(rope.val.children[k])
-    }
-
-    predicate minChildren(rope: Rope<T>)
-      reads rope
-    {
-      match rope.val
-      case Leaf(t) => true
-      case InternalNode(children) => |rope.val.children| >= min && forall k: int :: 0 <= k < |rope.val.children| ==> minChildren(rope.val.children[k])
-    }
-
-  }
-}
-
-
-
-
-
-datatype Rope<T> = Leaf(value: T) | Node(children: seq<Rope<T>>)
-
-function sum<T>(q: seq<Rope<T>>): int
-  requires |q| > 0
-{
-  if |q| == 1 then toList(1, q[0])
-  else toList(1, q[0]) + sum(q[1..])
-}
-
-
-function toList(d: int, t: Rope): int
-  decreases t
-{
-  match t
-  case Leaf(v) => d
-  case Node(children) =>
-    if |children| <= 0 then d
-    else sum(children)
-}
-
-
-
-
-
-
-
-
-predicate childCount(rope: Rope<T>)
-  reads rope
-{
-  match rope
-  case Leaf(t) => true
-  case
-}
-
-
-
-
-
-
-
-lemma countLemma(rope: Rope<T>, i: int)
-   requires i >= 0 && i < 5
-   ensures rope.Node? && (LeafCount(Node(rope.children[0..i-1], i - 1) + LeafCount(rope.children[i], 1) == LeafCount(rope, i)
-{
-
-}
-
-datatype Rope<T> = Leaf(value: T) | Node(children: seq<Rope<T>>)
-
-function rec(t: Rope): seq<int> {
-  match t
-  case Leaf(v) => 1
-  case Node(children) =>
-    if |children| <= 0 then 1
-    else toList(d+1, children[0]) + toList(d+1, Node(children[1..]))
-}
-
-function toList(d: int, t: Rope): seq<int>
-  decreases t
-{
-  match t
-  case Leaf(v) => [d]
-  case Node(children) =>
-    if |children| == 0 then [d]
-    else toList(d+1, children[0]) + toList(d+1, Node(children[1..]))
-}
-
-
-function LeafCount<T>(rope: Rope<T>, i: int): int {
-    match rope
-    case Leaf(t) => 1
-    case Node(children) =>
-      if |children| == 0 || i == 0 then 0
-      else LeafCount(children[0], 5) + LeafCount(Node(children[1..]), i - 1)
-}
-
-
-
-lemma sumLemma(s: seq<int>, i: int)
-   requires i >= 0 && i < |s|
-   ensures (sum(s, i) + s[i]) == sum(s, i + 1)
-{
-
 }
